formal/lakefile.lean
@@ -1,7 +1,8 @@
-﻿import Lake
+import Lake
 open Lake DSL
 
 package reflexive_dsha where
   moreLeanArgs := #["-DautoImplicit=false"]
 
+@[default_target]
 lean_lib ReflexiveDSHA
